curien.v
@@ -4,9 +4,9 @@ Import ListNotations.
 Inductive closure := | close : tm → list closure → closure. 
 Definition env := list closure.
 
-Inductive step : closure → closure → Prop := 
+Inductive step : closure → closure → Type := 
   | abs : ∀ b e, step (close (lam b) e) (close (lam b) e)
-  | var : ∀ x e v c, nth x e c → step c v → step (close (var x) e) v
+  | var : ∀ x e v c, nth_error e x = Some c → step c v → step (close (var x) e) v
   | app : ∀ m n b e v mve, 
       step (close m e) (close (lam b) mve) → 
       step (close b (close n e::mve)) v → 
