curien_cem_name.v
@@ -1,0 +1,58 @@
+Require Import List curien cem_name util Unicode.Utf8.
+
+Inductive env_eq (h : heap) : curien.env → cem_name.env → Type := 
+  | env_eq_nil : ∀ l, env_eq h nil l
+  | env_eq_cons : ∀ t e e' l l' l'', 
+      lookup l h = Some (cl (cem_name.close t l') l'') → 
+      env_eq h e l' → 
+      env_eq h e' l'' → 
+      env_eq h (curien.close t e :: e') l
+  .
+
+Inductive close_eq (h : heap) : curien.closure → cem_name.closure → Type := 
+  | close_equiv : ∀ t e l, env_eq h e l → close_eq h (curien.close t e) (cem_name.close t l).
+
+Lemma nth_lookup : ∀ x h e l c, env_eq h e l → nth_error e x = Some c → 
+  sigT (λ l', sigT (λ c', prod (clu x l h = Some (l', c')) (close_eq h c c'))). 
+induction x; intros. 
+-  inversion H0. subst. unfold clu. inversion H. subst. inversion H2. subst. exists l.
+   exists (close t l'). split; auto. rewrite H1. reflexivity. inversion H2. subst. apply close_equiv.  assumption.  
+-  inversion H0. subst. inversion H. subst. inversion H2. subst. apply IHx with (c:=c) in H4.
+   destruct H4. destruct s. exists x0. exists x1. simpl. rewrite H1. assumption. assumption. 
+Qed. 
+
+Lemma env_eq_fresh : ∀ x c h e l, env_eq h e l → x ∉ domain h → env_eq ((x,c)::h) e l. 
+intros. induce H; intros. constructor. apply env_eq_cons with (l':=l')
+(l'':=l''). unfold lookup. simpl.  destruct (PeanoNat.Nat.eqb l x) eqn:elx.
+symmetry in elx. apply EqNat.beq_nat_eq in elx. subst. apply lookup_domain in
+e0. apply H1 in e0.  inversion e0. unfold lookup in e0. assumption. apply
+IHenv_eq1. assumption. apply IHenv_eq2. assumption. 
+Qed.
+
+Lemma env_eq_step : ∀ h h' c v e l, cem_name.step (conf h c) (conf h' v) → env_eq h e l → env_eq h' e l.
+intros. induce X. 
+- invert H2. invert H1. apply IHX with (h0:=h) (c:=M) (v:=v0); auto. 
+- invert H2. invert H1. assumption. 
+- invert H2. invert H1. specialize (IHX1 _ _ _ _ e0 l H eq_refl eq_refl). apply
+  env_eq_fresh with (x:=f) (c:=cl (close N e) ne) in IHX1. specialize (IHX2 _ _
+  _ _ e0 l IHX1 eq_refl eq_refl). assumption. assumption. Qed.
+
+Theorem step_eq : ∀ h c c' v, close_eq h c c' → curien.step c v → 
+  sigT (λ co, match co with conf h' v' => prod (cem_name.step (conf h c') co) (close_eq h' v v') end). 
+intros. induce H0; intros. 
+- exists (conf h c'). inversion H. subst. split. constructor. assumption. 
+- destruct c'. inversion H. subst. apply (nth_lookup x h e cl_en c H2) in e0. 
+  destruct e0. destruct s. destruct p. specialize (IHstep h x1 c0). destruct
+  IHstep. destruct x2. destruct y. apply Id with (Ψ:=conf_h) (v:=conf_c) in e0.
+  exists (conf conf_h conf_c). split; auto. assumption. 
+- inversion H. subst.  specialize (IHstep1 h (close m l)). destruct IHstep1.
+  constructor; auto.  destruct x.  destruct y.  inversion c. subst. destruct
+  fresh with (l:=domain (conf_h)). specialize (IHstep2 ((x, cl (close n l)
+  l0)::conf_h) (close b x)). destruct IHstep2. constructor. apply env_eq_cons
+  with (l':=l) (l'':=l0). unfold lookup. simpl. rewrite PeanoNat.Nat.eqb_refl.
+  reflexivity. apply env_eq_fresh. apply env_eq_step with (h:=h) (c:=close m l)
+  (v:=close (db.lam b) l0). assumption. assumption. assumption. apply
+  env_eq_fresh. assumption. assumption. exists x0. destruct x0. split. apply
+  App with (B:=b) (Ψ:=conf_h) (f:=x) (ne:= l0). assumption. assumption.
+  destruct y. assumption. destruct y. assumption.  
+Qed. 
