set.v
@@ -1,0 +1,13 @@
+(* Library for Finite Sets *)
+Require Import List Basics.
+
+Definition set := list. 
+
+Fixpoint subset {A} (l : list A) (m: list A) : Prop := match l with
+  | nil => True
+  | cons x xs => In x m /\ subset xs m
+  end.
+
+Definition subset' {A} (l m : list A) : Prop := forall a, In a l -> In a m.
+
+
